Then
$$A_iA^i = {A^0}^2 + \va{A}^2$$

\paragraph{Transformation of 4-vector}
$$A^0 = \frac{{A^0}' + \frac{v}{c}{A^1}'}{\sqrt{1-\frac{v^2}{c^2}}}$$
$$A^1 = \frac{{A^1}' + \frac{v}{c}{A^0}'}{\sqrt{1-\frac{v^2}{c^2}}}$$

For covariant vector
$$\phi = \frac{{A^0}' - \frac{v}{c}{A^1}'}{\sqrt{1-\frac{v^2}{c^2}}}$$
$$A^1 = \frac{{A^1}' - \frac{v}{c}{A^0}'}{\sqrt{1-\frac{v^2}{c^2}}}$$

We can write in matrix form
$$A^i = L_j^i {A^j}'$$
\paragraph{Tensor}
Example of tensor wold be $A^iA^j$. To apply transform on tensor, we apply 
$$T^{lm} = L_{i}^l L_j^m {T'}^{ij}$$
\paragraph{Example}
$$\dd{s^2} = \dd{x_i} \dd{x^i} = c^2\dd{t^2} - (\dd{\va{r}})^2 = c^2\dd{t^2} \qty(1-\frac{\va{v}^2}{c^2}) \Rightarrow \dd{s} = \dd{t} \sqrt{1+\frac{v^2}{c^2}}$$
We define velocity
$$u^i = \dd{x^i}{s} = \qty(\frac{c\dd{t}}{c\dd{t}\sqrt{1-\frac{v^2}{c^2}}}, \frac{\dd{r}}{c\dd{t}\sqrt{1-\frac{v^2}{c^2}}}) = \qty(\frac{c\dd{t}}{c\dd{t}\sqrt{1-\frac{v^2}{c^2}}}, \frac{\dd{r}}{c\dd{t}\sqrt{1-\frac{v^2}{c^2}}}) = \qty(\frac{1}{\sqrt{1-\frac{v^2}{c^2}}}, \frac{\va{v}}{c\sqrt{1-\frac{v^2}{c^2}}})$$

Note that
$$u_iu^i = \dv{x^i}{s}\dv{x_i}{s} = \frac{\dd{x_i}\dd{x^i}}{\dd{s^2}}  = \frac{\dd{s^2}}{\dd{s^2}} = 1$$

Now define 4-vector of energy and momentum $p^i = mcu^i$. Then
$$p^y = \frac{m\dd{y}}{\dd{s}}$$
is conserved in all frames of reference.

\paragraph{Lagrangian of particle in electromagnetic field}
$$S =\int \mathcal{L}(t) \dd{t}$$
$$\mathcal{L}_{free} = -mc^2\sqrt{1-\frac{v^2}{c^2}}$$
Note that $\mathcal{L} \dd{t}$ is $\dd{s}$, which is invariant.

$$\mathcal{L} = -mc^2\sqrt{1-\frac{v^2}{c^2}} - q\phi +\frac{q}{c}\va{A} \vdot \va{v}$$

Then generalized momentum:
$$\va{P} = \pdv{\mathcal{L}}{\va{v}} =\underbrace{ \frac{m\va{v}}{\sqrt{1-\frac{v^2}{c^2}}}}_{\va{P}_0} + \frac{q}{c}\va{A}$$
And Hamiltonian, or energy
$$\mathcal{H}= \va{v} \pdv{\mathcal{L}}{\va{v}}  - \mathcal{L} =  \frac{mc^2}{\sqrt{1-\frac{v^2}{c^2}}} + q\phi$$

Then movement equations are
$$\dv{t} \pdv{\mathcal{L}}{\va{v}} - \pdv{\mathcal{L}}{\va{r}} = 0$$
$$\dv{t} \qty(\va{P}_0+\frac{q}{c}\va{A}) = \frac{q}{c} \grad(\va{A} \vdot \va{v}) - q\grad{\phi}$$
$$\dv{\va{A}}{t} = \pdv{\va{A}}{t} + (\va{v} \vdot \grad)\va{A}$$
$$\frac{q}{c}\grad(\va{A} \vdot \va{v}) = \frac{q}{c} \qty(\va{v} \vdot \grad) \va{V} + \frac{q}{c} v \cross \qty(\curl{\va{A}})$$
$$\dv{P_0}{t} = -\frac{q}{c} \pdv{\va{A}}{t} - q\grad{\phi} + \frac{q}{c} \grad(\va{A} \vdot \va{v})$$

Define
$$\va{B} = \curl{\va{A}}$$
and
$$\va{E} = -\frac{1}{c} \pdv{\va{A}}{t} - \grad{\phi}$$
in this case we get Faraday's law:
$$\curl{\va{E}} = -\frac{1}{c} \pdv{t} \va{B}$$
\paragraph{Relativity}
$$\int \mathcal{L} \dd{t} = \int \qty[-mc\dd{s} -\frac{q}{c} A_i \dd{x^i}]$$
$$A_i\dd{x^i} =A_0\dd{x^0} + \va{A} \vdot \dd{\va{r}} = c\phi \dd{t} - \va{A} \vdot \va{v}\dd{t} $$
$$\delta S = 0 \Rightarrow -\int \qty[-mc^2 \frac{\dd{x_i}\dd{\delta x^i}}{\dd{s}} + \frac{q}{c} A_i \dd{\delta x^i} + \frac{q}{c} \delta A_i \dd{x^i}] = 0$$
Now
$$\delta A_i = \pdv{A_i}{x^k}\delta x^k$$
After manipulations we get
$$\delta S = \int \qty[mc\dv{u_i}{s} - \frac{q}{c}\qty(\pdv{A_k}{x_i} - \pdv{A_i}{x^k})] \delta x^i \dd{s} = 0$$
Define
$$F_{ik} = \pdv{A_k}{x_i} - \pdv{A_i}{x^k} $$
and movement equation 
$$m\dv{u_i}{s} = \frac{q}{c} F_{ik} u^k$$
$$F = \begin{pmatrix}
0&E_x&E_y&E_z\\
-E_x&0&-B_z&B_y\\
-E_y&B_z&0&-B_x\\
-E_z&-B_y&-B_x&0
\end{pmatrix}$$
or, rather
$$F_{ik} = \qty(\va{E}, \va{B})$$
and contravarient
$$F^{ik} = \qty(-\va{E}, \va{B})$$
\paragraph{Example}
For $i=0$:
$$mc \dv{u^0}{s} = \frac{q}{c} F^{0k}u_k = \frac{q}{c} (-E_x)\frac{-v_x}{\sqrt{1-\frac{v^2}{c^2}}}+\frac{q}{c} (-E_y)\frac{-v_y}{\sqrt{1-\frac{v^2}{c^2}}}+\frac{q}{c} (-E_z)\frac{-v_z}{\sqrt{1-\frac{v^2}{c^2}}}$$
$$\dd{t} \frac{mc^2}{\sqrt{1-\frac{v^2}{c^2}}} = q \va{E} \vdot \va{v}$$
i.e.
$$\frac{mc^2}{\sqrt{1-\frac{v^2}{c^2}}} +q\Phi = \text{const}$$
which is energy conservation law.